Sure, here are the answers to the algebra problems:

1. Solution:

\begin{align*}
3(x-4)-2(x+3)&=7\\
3x-12-2x-6&=7\\
x&=25
\end{align*}

Therefore, the solution is x=25.

2. Solution:

\[3x^3+2x^2-5x^3+4x-6=-2x^3+2x^2+4x-6\]

Therefore, the simplified expression is \(-2x^3+2x^2+4x-6\).

3. Solution:

\[2x^2+5x-12=(2x-3)(x+4)\]

Therefore, the factored expression is \((2x-3)(x+4)\).

4. Solution:

\begin{align*}
5x+9&<3x+17\\
2x&<8\\
x&<4
\end{align*}

Therefore, the solution is x < 4.

5. Solution:

Solving the first equation for y, we get:
\[y=7-x\]

Substitute this value of y in the second equation to get:
\[2x-(7-x)=5\]
\[3x=12\]
\[x=4\]

Substitute this value of x in the first equation to get:
\[y=7-4=3\]

Therefore, the solution is (4,3).